ENHANCEMENT reworking ptsto
- more definitions & automation based on _at and _atP
- ported local-scope and class to _at

theories/Sem/PLogic.v
@@ -12,54 +12,153 @@ From Cpp Require Import Ast.
 
 From Cpp.Sem Require Import Logic Semantics.
 
-(* todo(gmm): these can be moved somewhere more generic *)
-Class Affine (P : mpred) : Prop :=
-{ can_dup : P |-- P ** P }.
-Class Droppable (P : mpred) : Prop :=
-{ can_drop : P |-- empSP }.
+Local Open Scope string_scope.
 
+(* todo(gmm): these can be moved somewhere more generic *)
+Class Affine {L : Type} {LL : ILogicOps L} {LS : BILogicOps L} (P : L) : Prop :=
+{ can_dup : P |-- P ** P }.
+Class Droppable {L : Type} {LL : ILogicOps L} {LS : BILogicOps L} (P : L) : Prop :=
+{ can_drop : P |-- empSP }.
 
 (* representations are predicates over a location, they should be used to
  * assert propreties of the heap
  *)
-Definition Rep : Type := forall addr : val, mpred.
+(* todo(gmm): `addr : val` -> `addr : ptr` *)
+Record Rep : Type :=
+  { repr : forall addr : val, mpred }.
+
+Global Instance ILogicOps_Rep : ILogicOps Rep :=
+{ lentails P Q := forall a, P.(repr) a |-- Q.(repr) a
+; ltrue := {| repr _ := ltrue |}
+; lfalse := {| repr _ := lfalse |}
+; land  P Q := {| repr a := land (P.(repr) a) (Q.(repr) a) |}
+; lor   P Q := {| repr a := lor (P.(repr) a) (Q.(repr) a) |}
+; limpl P Q := {| repr a := limpl (P.(repr) a) (Q.(repr) a) |}
+; lforall T P := {| repr a := lforall (fun v : T => (P v).(repr) a) |}
+; lexists T P := {| repr a := lexists (fun v : T => (P v).(repr) a) |}
+}.
+Global Instance ILogic_Rep : ILogic Rep.
+Admitted.
+Global Instance BILogicOps_Rep : BILogicOps Rep :=
+{ empSP := {| repr _ := empSP |}
+; sepSP P Q := {| repr a := sepSP (P.(repr) a) (Q.(repr) a) |}
+; wandSP P Q := {| repr a := wandSP (P.(repr) a) (Q.(repr) a) |}
+}.
+Global Instance BILogic_Rep : BILogic Rep.
+Admitted.
+
+
 (* locations are predicates over a location and are used to do address
  * arithmetic.
  * - note(gmm): they are always computable from the program except for when
- *   they use field and the layout of a class is non-standard or when they
+ *   they use field and the layout of a non-standard class or when they
  *   mention local variables.
  *)
 Record Loc : Type :=
-{ addr_of : forall addr : val, mpred }.
+  { addr_of : forall addr : val, mpred }.
+Global Instance ILogicOps_Loc : ILogicOps Loc :=
+{ lentails P Q := forall a, P.(addr_of) a |-- Q.(addr_of) a
+; ltrue := {| addr_of _ := ltrue |}
+; lfalse := {| addr_of _ := lfalse |}
+; land  P Q := {| addr_of a := land (P.(addr_of) a) (Q.(addr_of) a) |}
+; lor   P Q := {| addr_of a := lor (P.(addr_of) a) (Q.(addr_of) a) |}
+; limpl P Q := {| addr_of a := limpl (P.(addr_of) a) (Q.(addr_of) a) |}
+; lforall T P := {| addr_of a := lforall (fun v : T => (P v).(addr_of) a) |}
+; lexists T P := {| addr_of a := lexists (fun v : T => (P v).(addr_of) a) |}
+}.
+Global Instance ILogic_Loc : ILogic Loc.
+Admitted.
+Global Instance BILogicOps_Loc : BILogicOps Loc :=
+{ empSP := {| addr_of _ := empSP |}
+; sepSP P Q := {| addr_of a := sepSP (P.(addr_of) a) (Q.(addr_of) a) |}
+; wandSP P Q := {| addr_of a := wandSP (P.(addr_of) a) (Q.(addr_of) a) |}
+}.
+Global Instance BILogic_Loc : BILogic Loc.
+Admitted.
+
+
+
+Record Offset : Type :=
+  { offset : forall base new : val, mpred }.
+
+Global Instance ILogicOps_Offset : ILogicOps Offset :=
+{ lentails P Q := forall a b, P.(offset) a b |-- Q.(offset) a b
+; ltrue := {| offset _ := ltrue |}
+; lfalse := {| offset _ := lfalse |}
+; land  P Q := {| offset a := land (P.(offset) a) (Q.(offset) a) |}
+; lor   P Q := {| offset a := lor (P.(offset) a) (Q.(offset) a) |}
+; limpl P Q := {| offset a := limpl (P.(offset) a) (Q.(offset) a) |}
+; lforall T P := {| offset a := lforall (fun v : T => (P v).(offset) a) |}
+; lexists T P := {| offset a := lexists (fun v : T => (P v).(offset) a) |}
+}.
+Global Instance ILogic_Offset : ILogic Offset.
+Admitted.
+Global Instance BILogicOps_Offset : BILogicOps Offset :=
+{ empSP := {| offset _ _ := empSP |}
+; sepSP P Q := {| offset a b := sepSP (P.(offset) a b) (Q.(offset) a b) |}
+; wandSP P Q := {| offset a b := wandSP (P.(offset) a b) (Q.(offset) a b) |}
+}.
+Global Instance BILogic_Offset : BILogic Offset.
+Admitted.
+
+
+
 
 Definition LocEq (l1 l2 : Loc) : Prop :=
   forall x y, l1.(addr_of) x //\\ l2.(addr_of) y |-- [| x = y |].
 
-Definition _eq (a : val) : Loc :=
-{| addr_of p := [| p = a |] |}.
-Theorem _eq_LocEq : forall a b, LocEq (_eq a) (_eq b) -> a = b.
-Proof. unfold LocEq, _eq. intros.
-       simpl in *.
-       specialize (H a b).
-       admit.
-Admitted.
+Class Dup_Loc (l : Loc) : Prop :=
+  { can_dupL : l |-- l ** l }.
 
+(* absolute locations *)
+Definition _eq (a : val) : Loc :=
+  {| addr_of p := [| p = a |] |}.
+
+(* note(gmm): this is *not* duplicable *)
 Definition _local (r : region) (x : ident) : Loc.
 Admitted.
 Axiom _local_det : forall r x, LocEq (_local r x) (_local r x).
 
-Definition _field (f : field) (base : Loc) : Loc.
-Admitted.
-Axiom Proper__field : forall {f}, Proper (LocEq ==> LocEq) (_field f).
+Definition _this (r : region) : Loc :=
+  _local r "#this".
 
-Definition _sub (t : type) (i : Z) (base : Loc) : Loc.
+
+Definition _global (x : globname) : Loc.
 Admitted.
-Axiom Proper__sub : forall t i, Proper (LocEq ==> LocEq) (_sub t i).
+
+(* offsets *)
+Definition _field (f : field) : Offset.
+Admitted.
+
+Definition _sub (t : type) (i : Z) : Offset.
+Admitted.
 
 (* this represents static_cast *)
-Definition _super (from to : type) (base : Loc) : Loc.
+Definition _super (from to : type) : Offset.
 Admitted.
-Axiom Proper__super : forall from to, Proper (LocEq ==> LocEq) (_super from to).
+
+Definition _id : Offset :=
+  {| offset a b := embed (a = b) |}.
+Definition _dot (o1 o2 : Offset) : Offset :=
+  {| offset a c := Exists b, o1.(offset) a b ** o2.(offset) b c |}.
+
+Definition _offsetL (o : Offset) (l : Loc) : Loc :=
+  {| addr_of a := Exists a', o.(offset) a' a ** l.(addr_of) a' |}.
+Lemma _offsetL_dot : forall o1 o2 l,
+    _offsetL o2 (_offsetL o1 l) -|- _offsetL (_dot o1 o2) l.
+Proof.
+  unfold _offsetL, _dot; simpl.
+  constructor; simpl; intros; Discharge.discharge fail fail idtac.
+Qed.
+
+Definition _offsetR (o : Offset) (r : Rep) : Rep :=
+  {| repr a := Exists a', o.(offset) a a' ** r.(repr) a' |}.
+Lemma _offsetR_dot : forall o1 o2 l,
+    _offsetR o1 (_offsetR o2 l) -|- _offsetR (_dot o1 o2) l.
+Proof.
+  unfold _offsetL, _dot; simpl.
+  constructor; simpl; intros; Discharge.discharge fail fail idtac.
+Qed.
 
 
 
@@ -80,7 +179,7 @@ Parameter local_addr : region -> ident -> Loc.
 
 (* heap points to *)
 (* note(gmm): this needs to support fractional permissions and other features *)
-Parameter ptsto : val -> Rep.
+Parameter ptsto : forall addr value : val, mpred.
 
 
 
@@ -108,82 +207,176 @@ Inductive path : Type :=
 | p_cast (from to : type)  (_ : path) (* parent-class offset, i.e. static_cast *)
 | p_sub  (_ : type) (_ : val) (_ : path).
 
-Fixpoint pathD (p : path) (l : Loc) : Loc :=
+Fixpoint pathD (p : path) : Offset :=
   match p with
-  | p_done => l
-  | p_dot f p => pathD p (_field f l)
-  | p_cast from to p => pathD p (_super (drop_qualifiers from) (drop_qualifiers to) l)
+  | p_done => _id
+  | p_dot f p => _dot (_field f) (pathD p)
+  | p_cast from to p =>
+    _dot (_super (drop_qualifiers from) (drop_qualifiers to)) (pathD p)
   | p_sub t v p =>
-    {| addr_of a := Exists i : Z,
+    {| offset b a := Exists i : Z,
          [| Vint i = v |] //\\
-         (pathD p (_sub (drop_qualifiers t) i l)).(addr_of) a |}
+         (_dot (_sub (drop_qualifiers t) i) (pathD p)).(offset) b a |}
   end.
 
 Require Import Cpp.Auto.Discharge.
 
-Lemma pathD_det : forall p l1 l2,
-    LocEq l1 l2  -> LocEq (pathD p l1) (pathD p l2).
+(* Lemma pathD_det : forall p l1 l2, *)
+(*     LocEq l1 l2  -> LocEq (pathD p l1) (pathD p l2). *)
+(* Proof. *)
+(*   induction p; simpl; intros; eauto. *)
+(*   { eapply IHp. eapply Proper__field; eauto. } *)
+(*   { eapply IHp. eapply Proper__super. eauto. } *)
+(*   { red. simpl. intros. *)
+(*     rewrite landexistsDL1; eapply lexistsL; intro. *)
+(*     rewrite landexistsDL2; eapply lexistsL; intro. *)
+(*     unfold only_provable. *)
+(*     admit. } *)
+(* Admitted. *)
+
+
+(* Definition _addr (base : val) (p : path) : Loc := *)
+(*   pathD p (_eq base). *)
+
+Notation "a &~ b" := (a.(addr_of) b) (at level 30, no associativity).
+
+(* Theorem _addr_det : forall p b a1 a2, *)
+(*     _addr b p @@ a1 ** _addr b p @@ a2 |-- _addr b p @@ a1 ** [| a1 = a2 |]. *)
+(* Proof. Admitted. *)
+
+Class Duplicable_Offset (o : Offset) : Prop :=
+  { dup_offset : o |-- o ** o }.
+Arguments dup_offset {_ _}.
+
+Global Instance Duplicable_offset o {Do : Duplicable_Offset o} a b : Affine (offset o a b).
 Proof.
-  induction p; simpl; intros; eauto.
-  { eapply IHp. eapply Proper__field; eauto. }
-  { eapply IHp. eapply Proper__super. eauto. }
-  { red. simpl. intros.
-    rewrite landexistsDL1; eapply lexistsL; intro.
-    rewrite landexistsDL2; eapply lexistsL; intro.
-    unfold only_provable.
-    admit. }
-Admitted.
-
-
-Definition _addr (base : val) (p : path) : Loc :=
-  pathD p (_eq base).
-
-Notation "a @@ b" := (a.(addr_of) b) (at level 30, no associativity).
-
-Theorem _addr_det : forall p b a1 a2,
-    _addr b p @@ a1 ** _addr b p @@ a2 |-- _addr b p @@ a1 ** [| a1 = a2 |].
-Proof. Admitted.
-
-
-(*
-Parameter Affine__addr : forall b p a, Affine (_addr b p a).
-Parameter Droppable__addr : forall b p a, Droppable (_addr b p a).
-*)
-
-Definition _atP (base : val) (p : path) (P : Rep) : mpred :=
-  Exists addr, (_addr base p) @@ addr ** P addr.
+  constructor. eapply dup_offset.
+Qed.
 
 
 Definition _at (base : Loc) (P : Rep) : mpred :=
-  Exists addr, base @@ addr ** P addr.
+  Exists a, base.(addr_of) a ** P.(repr) a.
+
+Definition _atP (base : Loc) (p : Offset) (P : Rep) : mpred :=
+  _at (_offsetL p base) P.
+
+Theorem _atP_at : forall b p P,
+    _atP b p P -|- _at (_offsetL p b) P.
+Proof. reflexivity. Qed.
+
+Arguments can_dup {_ _ _} _ {_}.
+
+Lemma offset_consolidate p a b c :
+  offset p a b ** offset p a c |-- offset p a b ** [| b = c |].
+Proof. Admitted.
+
+Lemma _atP_sepSP : forall b p P Q,
+    Duplicable_Offset p ->
+    _atP (_eq b) p (P ** Q) -|- _atP (_eq b) p P ** _atP (_eq b) p Q.
+Proof.
+  intros; split.
+  { unfold _atP, _at, _eq, _offsetL. simpl.
+    lift_ex_l fail.
+    rewrite (can_dup (offset p x0 x)).
+    Discharge.discharge fail fail idtac.
+    eapply provable_star; auto.
+    eapply only_provable_only; eauto. }
+  { unfold _atP, _at, _eq, _offsetL. simpl.
+    lift_ex_l fail.
+    subst.
+    transitivity ((offset p b x1 ** offset p b x) ** repr P x ** repr Q x1).
+    - Discharge.discharge fail fail idtac.
+    - rewrite offset_consolidate.
+      Discharge.discharge fail fail idtac.
+      subst.
+      Discharge.discharge fail fail idtac.
+      eapply only_provable_only; eauto. }
+Qed.
+
+Lemma _atP_exists : forall b p T (P : T -> _),
+    _atP b p (lexists P) -|- Exists x : T, _atP b p (P x).
+Proof.
+  unfold _atP, _at; simpl.
+  split.
+  { Discharge.discharge fail fail idtac. }
+  { Discharge.discharge fail fail idtac. }
+Qed.
+
+Lemma _atP_offsetR : forall b p o P,
+    _atP b p (_offsetR o P) -|- _atP b (_dot p o) P.
+Proof.
+  unfold _atP, _at, _offsetR; simpl. split.
+  { Discharge.discharge fail fail idtac. }
+  { Discharge.discharge fail fail idtac. }
+Qed.
+
+
+
 
 (* this should probably be split up into a bunch of simpler definitions, e.g.
  * - `tint (size : nat) : N -> Rep`
  * - `tuint (size : nat) : N -> Rep`
  * - ...etc...
  *)
+Definition tint (sz : nat) (v : Z) : Rep :=
+  {| repr := fun addr =>
+               ptsto addr (Vint v) **
+               [| has_type (Vint v) (Tint (Some sz) true) |] |}.
+Definition tuint (sz : nat) (v : Z) : Rep :=
+  {| repr := fun addr =>
+               ptsto addr (Vint v) **
+               [| has_type (Vint v) (Tint (Some sz) false) |] |}.
+Definition tptr (ty : type) (p : ptr) : Rep :=
+  {| repr := fun addr => ptsto addr (Vptr p) |}.
+Definition tref (ty : type) (p : val) : Rep :=
+  {| repr addr := [| addr = p |] |}.
+
+
 Definition tprim (ty : type) (v : val) : Rep :=
-  fun addr => ptsto addr v ** [| has_type v (drop_qualifiers ty) |].
+  {| repr := fun addr => ptsto addr v ** [| has_type v (drop_qualifiers ty) |] |}.
+Axiom tprim_tint : forall sz v,
+    tprim (Tint (Some sz) true) (Vint v) -|- tint sz v.
+Axiom tprim_tuint : forall sz v,
+    tprim (Tint (Some sz) false) (Vint v) -|- tuint sz v.
+Axiom tprim_tptr : forall ty p,
+    tprim (Tpointer ty) (Vptr p) -|- tptr (drop_qualifiers ty) p.
 
-Definition uninit (ty : type) : Rep := fun addr =>
-  Exists bits,
-    (* with_genv (fun env => [| size_of env ty size |]) ** *)
-    tprim ty bits addr.
+Definition uninit (ty : type) : Rep :=
+  {| repr := fun addr =>
+               Exists bits,
+               (* with_genv (fun env => [| size_of env ty size |]) ** *)
+               (tprim ty bits).(repr) addr |}.
 
-Definition tany (t : type) : Rep := fun addr =>
-  Exists v, [| has_type v t |] ** tprim t v addr.
+Definition tany (t : type) : Rep :=
+  {| repr := fun addr =>
+               Exists v, [| has_type v t |] ** (tprim t v).(repr) addr |}.
 
 (* this isn't really necessary, we should simply drop it and write
  * predicates in this way to start with
  *)
 Definition tinv {model} (Inv : val -> model -> mpred) (m : model) : Rep :=
-  fun addr => Inv addr m.
+  {| repr := fun addr => Inv addr m |}.
 
-Lemma val_uninit : forall t v, tprim t v |-- uninit t.
+Lemma tint_uninit : forall sz v, tint sz v |-- uninit (Tint (Some sz) true).
+Admitted.
+Lemma tuint_uninit : forall sz v, tuint sz v |-- uninit (Tint (Some sz) false).
+Admitted.
+Lemma tptr_uninit : forall ty p, tptr ty p |-- uninit (Tpointer ty).
+Admitted.
+Lemma tprim_uninit : forall t v, tprim t v |-- uninit t.
 Proof. Admitted.
 
 Lemma val_any : forall t v, tprim t v |-- tany t.
 Proof. Admitted.
+
+Lemma refine_tprim_ptr : forall p ty v F Q,
+    (forall pt, Vptr pt = v ->
+           _at p (tptr (drop_qualifiers ty) pt) ** F |-- Q) ->
+    _at p (tprim (Tpointer ty) v) ** F |-- Q.
+Proof.
+  unfold _at, tprim.
+  intros; simpl.
+Admitted.
 
 Definition _at_cancel : forall a (V V' : Rep) P Q,
     V |-- V' ->
@@ -191,22 +384,21 @@ Definition _at_cancel : forall a (V V' : Rep) P Q,
     _at a V ** P |-- _at a V' ** Q.
 Proof. Admitted.
 
-Definition tlocal_at (r : region) (ty : type) (l : ident) (a : val) (v : val) : mpred :=
-  _local r l @@ a **
-  [| has_type a (Tpointer ty) |] **
-  _at (_eq a) (tprim ty v).
+Definition tlocal_at (r : region) (l : ident) (a : val) (v : Rep) : mpred :=
+  _local r l &~ a **
+  _at (_eq a) v.
 
-Definition tlocal (r : region) (ty : type) (x : ident) (v : val) : mpred :=
-  Exists a, tlocal_at r ty x a v.
+Definition tlocal (r : region) (x : ident) (v : Rep) : mpred :=
+  Exists a, tlocal_at r x a v.
 
-Lemma tlocal_at_tlocal : forall r ty x a v F F',
+Lemma tlocal_at_tlocal : forall r x a v F F',
     F |-- F' ->
-    tlocal_at r ty x a v ** F |-- tlocal r ty x v ** F'.
+    tlocal_at r x a v ** F |-- tlocal r x v ** F'.
 Proof.
   clear. unfold tlocal, tlocal_at.
   intros.
   rewrite H.
-  Discharge.discharge fail eauto.
+  Discharge.discharge ltac:(fail) fail eauto.
 Qed.
 
 Fixpoint uninitializedN (size : nat) (a : val) : mpred :=
@@ -214,33 +406,35 @@ Fixpoint uninitializedN (size : nat) (a : val) : mpred :=
   | 0 => empSP
   | S size => (Exists x, ptsto a x) ** uninitializedN size (offset_ptr a 1)
   end.
-Definition uninitialized (size : N) : val -> mpred :=
-  uninitializedN (BinNatDef.N.to_nat size).
+Definition uninitialized (size : N) : Rep :=
+  {| repr := uninitializedN (BinNatDef.N.to_nat size) |}.
 
-Definition uninitialized_ty (tn : type) (p : val) : mpred :=
+Definition uninitialized_ty (tn : type) : Rep :=
+{| repr := fun p : val =>
   Exists sz, with_genv (fun g => [| @size_of g tn sz |]) **
-                       uninitialized sz p.
+                       (uninitialized sz).(repr) p |}.
 
+Opaque uninitialized_ty.
 
+(*
 (* p is a path
  * P is a predicate over the resulting value
  *)
 Definition data (P : val -> mpred) (p : val -> mpred) : mpred.
 refine (Exists v, p v //\\ P v).
 Defined.
+*)
 
-Require Import Coq.Lists.List.
+(* Require Import Coq.Lists.List. *)
 
-Definition tptsto t a v :=
-  _at a (tprim (drop_qualifiers t) v).
+(* Definition tptsto t a v := *)
+(*   _at a (tprim (drop_qualifiers t) v). *)
 
-Definition tat_field (t : type) (base : val) (f : field) (v : val) : mpred :=
-  _atP base (p_dot f p_done) (tprim t v).
+(* Definition tat_field (t : type) (base : val) (f : field) (v : val) : mpred := *)
+(*   _atP base (p_dot f p_done) (tprim t v). *)
 
-
-
-Lemma tat_uninitialized
-  : forall t b f v F F',
-    F |-- F' ->
-    tat_field t b f v ** F |-- _atP b (p_dot f p_done) (uninit t).
-Proof. Admitted.
+(* Lemma tat_uninitialized *)
+(*   : forall t b f v F F', *)
+(*     F |-- F' -> *)
+(*     tat_field t b f v ** F |-- _atP b (p_dot f p_done) (uninit t). *)
+(* Proof. Admitted. *)
