tests/demo/A_hpp_spec.v
@@ -17,8 +17,8 @@ Definition A__foo_spec : function_spec' :=
   SFunction (Qmut T_int) (Qmut T_int :: nil)
       (fun x =>
          {| wpp_with := Z
-          ; wpp_pre := fun y => [| x = Vint y |] ** [| has_type (y + 6) T_int |]
-          ; wpp_post := fun y (r : val) => [| r = Vint (y + 6)%Z |]
+          ; wpp_pre y := [| x = Vint y |] ** [| has_type (y + 6) T_int |]
+          ; wpp_post y (r : val) := [| r = Vint (y + 6)%Z |]
           |}).
 
 Definition A__bar := "_ZN1A3barEi".
@@ -26,8 +26,8 @@ Definition A__bar_spec : function_spec' :=
   SFunction (Qmut T_int) (Qmut T_int :: nil)
       (fun x =>
          {| wpp_with := Z
-          ; wpp_pre := fun y => [| x = Vint y |] ** [| has_type (y + 7) T_int |]
-          ; wpp_post := fun y (r : val) => [| r = Vint (y + 7)%Z |]
+          ; wpp_pre y := [| x = Vint y |] ** [| has_type (y + 7) T_int |]
+          ; wpp_post y (r : val) := [| r = Vint (y + 7)%Z |]
           |}).
 
 Definition A_hpp_spec (resolve : _) :=
